Work on gallina and general model

src/named/GeneralModel.v
@@ -22,11 +22,13 @@ Local Notation mut_mod eq_sort eq_term wf_sort wf_term :=
       Model.wf_term := wf_term;
     |}.
 
+Section WithExp.
+
 Context {V : Type}
         {V_Eqb : Eqb V}
         {V_default : WithDefault V}
-        {exp : Type}
-        {default : exp}.
+        (exp : Type)
+        (default : exp).
 
 
 Notation named_list := (@named_list V).
@@ -59,8 +61,8 @@ Definition id_substable {B} (e : term) :=
 
 Definition ws_term args (e : term) :=
     (forall s, map fst s = args ->
-         forall s', (forall arg, In arg args -> named_list_lookup default s arg = named_list_lookup default s' arg) ->
-           e s = e s')
+         forall s', (forall arg, In arg args -> named_list_lookup default s' arg = named_list_lookup default s arg) ->
+           e s' = e s)
   /\ forall B, id_substable (B:=B) e.
 
 Instance substable_term : Substable0 term :=
@@ -75,269 +77,6 @@ Instance substable_sort : Substable term sort :=
     apply_subst := fun _ B => B;
     well_scoped := fun _ _ => True
   }.
-
-
-Ltac unfold_all :=
-  repeat (unfold apply_subst, inj_var, subst_lookup; simpl).
-
-Ltac cases x :=
-  case_eq x; intros;
-  match goal with
-  | [ H : eqb _ _ = true |- _ ] => apply eqb_eq in H; rewrite H
-  | [ H : eqb _ _ = false |- _ ] => apply eqb_neq in H
-  | _ => idtac
-  end.
-
-  Ltac if_refl :=
-    match goal with
-    | [ H : ?a = ?b |- (if eqb ?a ?b then _ else _) = _ ] => rewrite H
-    | [ H : ?b = ?a |- (if eqb ?a ?b then _ else _) = _ ] => rewrite H
-    | _ => idtac
-    end;
-    match goal with
-    | [ |- (if eqb ?a ?a then _ else _) = _ ] => replace (eqb a a) with (true); try (symmetry; apply eqb_refl)
-    | _ => idtac
-    end.
-
-  Lemma eqb_eq_eqb : forall (H1 H2 : Eqb V) (x y : V), eqb (Eqb:=H1) x y = eqb (Eqb:=H2) x y.
-    Proof.
-      intros.
-      case_eq (eqb x y); intros.
-      apply eqb_eq in H.
-      apply eqb_eq.
-      trivial.
-      apply eqb_neq in H.
-      apply eqb_neq.
-      trivial.
-Qed.
-
-  Lemma subst_var : forall (H : Eqb V) (s : named_list term) (x : V),
-      apply_subst s (inj_var x) = subst_lookup s x.
-  Proof.
-    intros.
-    unfold_all.
-    induction s; simpl; trivial.
-    unfold pair_map_snd.
-    destruct a.
-    assert (eqb (Eqb:=V_Eqb) x v = eqb (Eqb:=H) x v)by apply eqb_eq_eqb.
-    rewrite H0.
-    case (eqb x v); trivial.
-Qed.
-
-  Lemma lookup_found {A} : forall (l1 l2 : named_list A) d1 d2 (e : V), In e (map fst l1) -> named_list_lookup d1 (l1 ++ l2) e = named_list_lookup d2 l1 e.
-  Proof.
-    intros.
-    induction l1.
-    inversion H.
-    simpl in *.
-    destruct H; destruct a; simpl in *.
-    rewrite H.
-    assert (eqb e e = true).
-    apply eqb_eq.
-    trivial.
-    rewrite H0; simpl.
-    trivial.
-    case (eqb e v).
-    trivial.
-    apply IHl1.
-    apply H.
-Qed.
-
-  Lemma ws_term_append : forall (args : list V) (l1 l2 : named_list exp) (a : term),
-      ws_term args a -> args = map fst l1 -> a (l1 ++ l2) = a l1.
-  Proof.
-    intros.
-    unfold ws_term in  H.
-    symmetry in H0.
-    destruct H.
-    specialize (H l1 H0 (l1 ++ l2)).
-    symmetry.
-    apply H.
-    intros.
-    symmetry.
-    apply lookup_found.
-    rewrite <- H0 in H2; trivial.
-  Qed.
-
-  Lemma named_map_cons_eq {A B} : forall l (n : V) (e : A) (f : A -> B),
-      named_map f ((n, e) :: l) = (n, f e) :: named_map f l.
-  Proof.
-    trivial.
-  Qed.
-
-  Lemma named_map_fst {A B} : forall (l : named_list A) (f : A -> B), map fst l = map fst (named_map f l).
-    Proof.
-      intros.
-      induction l.
-      trivial.
-      destruct a.
-      rewrite named_map_cons_eq.
-      repeat rewrite map_cons.
-      simpl.
-      apply invert_eq_cons_cons.
-      constructor; trivial.
-    Qed.
-
-
-  Lemma named_map_fst' {A B C} : forall (l1 : named_list A) (l2 : named_list B) (f : B -> C), map fst l1 = map fst l2 -> map fst l1 = map fst (named_map f l2).
-    Proof.
-      intros; rewrite H.
-      apply named_map_fst.
-    Qed.
-   Lemma named_map_cmp {A B C} : forall (f : B -> C) (g : A -> B) h (l : named_list A), (forall x, f (g x) = h x) -> named_map f (named_map g l) = named_map h l.
-  Proof.
-    intros.
-    induction l.
-    trivial.
-    destruct a.
-    repeat rewrite named_map_cons_eq.
-    apply invert_eq_cons_cons.
-    constructor.
-    rewrite H; trivial.
-    trivial.
-Qed.
-
-  Ltac cleanup_ws_append :=
-    match goal with
-    | [H : ws_term _ ?a |- ws_term _ ?a] => apply H
-    | [ |- map fst _ = map fst (named_map _ _)] => repeat apply named_map_fst'; trivial
-    | _ => idtac
-    end.
-
-  Lemma subst_assoc0 : forall (s1 s2 : named_list term) (a : term),
-      ws_term (map fst s2) a -> apply_subst s1 (apply_subst s2 a) = apply_subst (subst_cmp s1 s2) a.
-  Proof.
-    intros.
-    unfold subst_cmp.
-    simpl.
-    unfold apply_subst in *.
-    apply functional_extensionality; intros.
-    repeat erewrite ws_term_append; cleanup_ws_append.
-    f_equal.
-    symmetry.
-    apply named_map_cmp.
-    trivial.
-Qed.
-  Lemma subst_id0 {B} : forall (c : named_list B) (a : term),
-      ws_term (map fst c) a -> apply_subst (id_subst c) a = a.
-  Proof.
-    intros.
-    destruct H.
-    unfold id_substable in H0.
-    specialize (H0 B c).
-    auto.
-Qed.
-
-  Lemma in_fst {A} : forall n (e : A) (l : named_list A), In (n, e) l -> In n (map fst l).
-  Proof.
-    intros.
-    induction l.
-    trivial.
-    inversion H; rewrite map_cons; simpl.
-    left.
-    rewrite H0.
-    trivial.
-    apply IHl in H0.
-    right.
-    trivial.
-Qed.
-    
-    
-  Lemma in_fst' {A} : forall n (e : A) (l1 : named_list A) (l2 : list V), map fst l1 = l2 -> In n l2 -> In n (map fst l1).
-  Proof.
-    intros.
-    rewrite H.
-    trivial.
-Qed.
-
-  Lemma strengthen_subst0 : forall (s : named_list term) (e a : term) (n : V),
-      ws_term (map fst s) a -> fresh n s ->
-      apply_subst ((n, e) :: s) a = apply_subst s a.
-  Proof.
-    intros.
-    unfold apply_subst.
-    apply functional_extensionality; intros.
-    symmetry; erewrite ws_term_append at 1; cleanup_ws_append.
-    remember (fun t => t x) as f.
-    pose proof (named_map_fst s f (A := (meta_subst -> exp))) as nmf.
-    symmetry in nmf.
-    destruct H.
-    specialize (H (named_map f s) nmf (named_map f ((n, e) :: s) ++ x)).
-    apply H.
-    intros.
-    unfold fresh in H0.
-    rewrite named_map_cons_eq.
-    case_eq (eqb arg n); intros.
-    apply eqb_eq in H3.
-    rewrite H3 in H2.
-    apply H0 in H2; contradiction.
-    simpl.
-    rewrite H3.
-    symmetry; apply lookup_found.
-    rewrite nmf; trivial.
-Qed.
-
-  Lemma fun_app_eq {A B} : forall (f g : A -> B) (a : A), f = g -> f a = g a.
-  Proof.
-    intros.
-    rewrite H.
-    trivial.
-  Qed.
-
-  Lemma well_scoped_subst0 : forall (args : list V) (s : named_list term) (a : term),
-      ws_subst args s ->
-      ws_term (map fst s) a ->
-      ws_term args (apply_subst s a).
-  Proof.
-    constructor; intros.
-    + unfold apply_subst.
-      repeat erewrite ws_term_append; cleanup_ws_append.
-      f_equal.
-      clear H0.
-      induction s.
-      trivial.
-      destruct a0.
-      repeat rewrite named_map_cons_eq.
-      destruct H.
-      destruct H0.
-      destruct H0.
-      specialize (H0 s0 H1 s' H2).
-      rewrite H0.
-      rewrite IHs; trivial.
-    + unfold id_substable.
-      intros.
-      unfold apply_subst.
-      apply functional_extensionality; intros.
-      repeat erewrite ws_term_append; cleanup_ws_append.
-      clear H0.
-      f_equal.
-      induction s.
-      trivial.
-      destruct a0.
-      repeat rewrite named_map_cons_eq.
-      destruct H.
-      destruct H0.
-      destruct H0.
-      unfold id_substable in H2.
-      specialize (H2 B c).
-      apply fun_app_eq with (a := x) in H2.
-      rewrite H2.
-      rewrite IHs; trivial.
-Qed.
-
-Instance substable_term_ok : Substable0_ok term.
-constructor; intros.
-- apply subst_var.
-- apply subst_assoc0; trivial.
-- apply subst_id0; trivial.
-- apply strengthen_subst0; trivial.
-- apply well_scoped_subst0; trivial.
-Qed.
-
-Instance substable_sort_ok : Substable_ok term sort.
-Proof.
-  constructor; intros; trivial.
-Qed.
 
 Definition ctx : Type := named_list sort.
 
@@ -355,22 +94,257 @@ Notation Model := (@Model V term sort).
 
 #[export] Instance model : Model := mut_mod eq_sort eq_term wf_sort wf_term.
 
+Ltac unfold_all :=
+  repeat (unfold apply_subst, inj_var, subst_lookup, pair_map_snd, wf_term, Substable.apply_subst in *; simpl in *).
+
+Ltac cases x :=
+  case_eq x; intros;
+  match goal with
+  | [ H : eqb _ _ = true |- _ ] => apply eqb_eq in H; rewrite H
+  | [ H : eqb _ _ = false |- _ ] => apply eqb_neq in H
+  | _ => idtac
+  end.
+
+  Ltac if_refl :=
+    match goal with
+    | [ H : ?a = ?b |- (if eqb ?a ?b then _ else _) = _ ] => rewrite H
+    | [ H : ?b = ?a |- (if eqb ?a ?b then _ else _) = _ ] => rewrite H
+    | [ H : ?a <> ?b |- (if eqb ?a ?b then _ else _) = _ ] => rewrite <- eqb_neq in H; rewrite H
+    | [ H : ?a = ?b |- _ = (if eqb ?a ?b then _ else _) _ ] => rewrite H
+    | [ H : ?b = ?a |- _ = (if eqb ?a ?b then _ else _) _ ] => rewrite H
+    | [ H : ?a <> ?b |- _ = (if eqb ?a ?b then _ else _) _ ] => rewrite <- eqb_neq in H; rewrite H
+    | _ => idtac
+    end;
+    match goal with
+    | [ |- (if eqb ?a ?a then _ else _) = _ ] => replace (eqb a a) with (true); try (symmetry; apply eqb_refl)
+    | [ |- _ = (if eqb ?a ?a then _ else _) _ ] => replace (eqb a a) with (true); try (symmetry; apply eqb_refl)
+    | _ => idtac
+    end.
+
+  Lemma named_map_fst {A B} : forall (l : named_list A) (f : A -> B), map fst l = map fst (named_map f l).
+    Proof.
+      intros.
+      induction l; simpl; trivial.
+      rewrite IHl.
+      unfold pair_map_snd; destruct a; simpl.
+      trivial.
+    Qed.
+
+
+  Lemma named_map_fst' {A B C} : forall (l1 : named_list A) (l2 : named_list B) (f : B -> C), map fst l1 = map fst l2 -> map fst l1 = map fst (named_map f l2).
+    Proof.
+      intros.
+      rewrite H.
+      apply named_map_fst.
+    Qed.
+
+Ltac model_crush :=
+  repeat
+    (intros;
+     unfold_all;
+     trivial;
+     match goal with
+     | [x : _ * _ |- _] => destruct x
+     | [|- (fun _ => _) = _] => apply functional_extensionality
+     | [|- (if ?a then _ else _) = _] => cases a; if_refl
+     | [|- _ = (if ?a then _ else _)] => cases a; if_refl
+     | [H : False |- _] => inversion H
+     | [H : _ /\ _ |- _] => destruct H
+     | [H : _ \/ _ |- _] => destruct H
+     | [|- _ /\ _] => constructor
+     | [H : ?a, H': ?a -> ?b |- _] => apply H' in H; clear H'
+     | [|- _ :: _ = _ :: _] => apply invert_eq_cons_cons
+     | [|- (_, _) = (_, _)] => apply pair_equal_spec
+     | [H : _ :: _ = _ :: _ |- _] => apply invert_eq_cons_cons in H
+     | [H : (_, _) = (_, _) |- _] => apply pair_equal_spec in H
+     | [H : _ = _ |- _] => try rewrite H
+     | [H : ws_term _ ?a |- ws_term _ ?a] => apply H
+     | [ |- map fst (named_map _ _) = map fst _] => symmetry
+     | [ |- map fst _ = map fst (named_map _ _)] => repeat apply named_map_fst'; trivial
+     | _ => idtac
+     end;
+     try rewrite <- named_map_fst;
+     if_refl
+    ).
+
+
+  Lemma eqb_eq_eqb : forall (H1 H2 : Eqb V) (x y : V), eqb (Eqb:=H1) x y = eqb (Eqb:=H2) x y.
+    Proof.
+      intros.
+      case_eq (eqb x y); intros.
+      apply eqb_eq in H.
+      apply eqb_eq.
+      trivial.
+      apply eqb_neq in H.
+      apply eqb_neq.
+      trivial.
+Qed.
+
+  Lemma subst_var : forall (H : Eqb V) (s : named_list term) (x : V),
+      apply_subst s (inj_var x) = subst_lookup s x.
+  Proof.
+    model_crush.
+    induction s; model_crush.
+Qed.
+
+  Lemma lookup_found {A} : forall (l1 l2 : named_list A) d1 d2 (e : V), In e (map fst l1) -> named_list_lookup d1 (l1 ++ l2) e = named_list_lookup d2 l1 e.
+  Proof.
+    model_crush.
+    induction l1; model_crush.
+    rewrite H in H0; contradict H0; apply eq_refl.
+Qed.
+
+  Lemma ws_term_append : forall (args : list V) (l1 l2 : named_list exp) (a : term),
+      ws_term args a -> map fst l1 = args -> a (l1 ++ l2) = a l1.
+  Proof.
+    model_crush.
+    apply H; model_crush.
+    apply lookup_found.
+    unfold ws_term in H.
+    rewrite <- H0 in H1; trivial.
+  Qed.
+
+  Lemma named_map_cons_eq {A B} : forall l (n : V) (e : A) (f : A -> B),
+      named_map f ((n, e) :: l) = (n, f e) :: named_map f l.
+  Proof.
+    trivial.
+  Qed.
+
+
+   Lemma named_map_cmp {A B C} : forall (f : B -> C) (g : A -> B) h (l : named_list A), (forall x, f (g x) = h x) -> named_map f (named_map g l) = named_map h l.
+  Proof.
+    model_crush.
+    induction l; model_crush.
+
+Qed.
+
+  Lemma subst_assoc0 : forall (s1 s2 : named_list term) (a : term),
+      ws_term (map fst s2) a -> apply_subst s1 (apply_subst s2 a) = apply_subst (subst_cmp s1 s2) a.
+  Proof.
+    model_crush.
+    repeat erewrite ws_term_append; model_crush.
+    f_equal.
+    symmetry.
+    apply named_map_cmp.
+    trivial.
+  Qed.
+
+  Lemma subst_id0 {B} : forall (c : named_list B) (a : term),
+      ws_term (map fst c) a -> apply_subst (id_subst c) a = a.
+  Proof.
+    intros.
+    destruct H.
+    unfold id_substable in H0.
+    specialize (H0 B c).
+    auto.
+Qed.
+
+  Lemma in_fst {A} : forall n (e : A) (l : named_list A), In (n, e) l -> In n (map fst l).
+  Proof.
+    intros.
+    induction l; model_crush.
+    left; trivial.
+    right; trivial.
+Qed.
+    
+    
+  Lemma in_fst' {A} : forall n (e : A) (l1 : named_list A) (l2 : list V), map fst l1 = l2 -> In n l2 -> In n (map fst l1).
+  Proof.
+    model_crush.
+Qed.
+
+  Lemma strengthen_subst0 : forall (s : named_list term) (e a : term) (n : V),
+      ws_term (map fst s) a -> fresh n s ->
+      apply_subst ((n, e) :: s) a = apply_subst s a.
+  Proof.
+    intros.
+    unfold apply_subst.
+    apply functional_extensionality; intros.
+    symmetry; erewrite ws_term_append at 1.
+    remember (fun t => t x) as f.
+    pose proof (named_map_fst s f (A := (meta_subst -> exp))) as nmf.
+    symmetry in nmf.
+    destruct H.
+    specialize (H (named_map f s) nmf (named_map f ((n, e) :: s) ++ x)).
+    symmetry; apply H.
+    intros.
+    unfold fresh in H0.
+    rewrite named_map_cons_eq.
+    case_eq (eqb arg n); intros.
+    apply eqb_eq in H3.
+    rewrite H3 in H2.
+    apply H0 in H2; contradiction.
+    simpl.
+    rewrite H3.
+    apply lookup_found.
+    rewrite nmf; trivial.
+    all: model_crush.
+Qed.
+
+  Lemma fun_app_eq {A B} : forall (f g : A -> B) (a : A), f = g -> f a = g a.
+  Proof.
+    model_crush.
+  Qed.
+
+  Lemma well_scoped_subst0 : forall (args : list V) (s : named_list term) (a : term),
+      ws_subst args s ->
+      ws_term (map fst s) a ->
+      ws_term args (apply_subst s a).
+  Proof.
+    model_crush.
+    constructor; model_crush.
+    + repeat erewrite ws_term_append; model_crush; model_crush.
+      f_equal.
+      clear H0.
+      induction s.
+      trivial.
+      destruct a0.
+      repeat rewrite named_map_cons_eq.
+      destruct H.
+      destruct H0.
+      destruct H0.
+      specialize (H0 s0 H1 s' H2).
+      rewrite H0.
+      rewrite IHs; trivial.
+    + unfold id_substable.
+      model_crush.
+      repeat erewrite ws_term_append; model_crush; model_crush.
+      clear H0.
+      f_equal.
+      induction s.
+      model_crush.
+      unfold ws_subst in H.
+      destruct a0.
+      destruct H.
+      destruct H0.
+      destruct H0.
+      unfold id_substable in H2.
+      specialize (H2 B c).
+      apply fun_app_eq with (a := x) in H2.
+      model_crush.
+Qed.
+
+Instance substable_term_ok : Substable0_ok term.
+constructor; intros.
+- apply subst_var.
+- apply subst_assoc0; trivial.
+- apply subst_id0; trivial.
+- apply strengthen_subst0; trivial.
+- apply well_scoped_subst0; trivial.
+Qed.
+
+Instance substable_sort_ok : Substable_ok term sort.
+Proof.
+  constructor;
+  model_crush.
+Qed.
+
+
 
   Lemma term_subst_id_eq {A} : forall (c : named_list A) n, apply_subst (with_names_from c (map inj_var (map fst c))) (inj_var n) = inj_var n.
     Proof.
-    intros.
-    unfold apply_subst in *.
-    apply functional_extensionality.
-    intros.
-    unfold inj_var in *.
-    induction c.
-    trivial.
-    destruct a.
-    simpl.
-    case_eq (eqb n v); intros.
-    apply eqb_eq in H.
-    rewrite H; trivial.
-    apply IHc.
+      model_crush.
+      induction c; model_crush.
   Qed.
 
   Lemma eq_term_subst : forall (c : ctx) (s1 s2 : named_list term)
@@ -381,52 +355,28 @@ Notation Model := (@Model V term sort).
                     eq_term c t [/s2 /] e1 [/s1 /] e2 [/s2 /].
     Proof.
       unfold eq_term in *.
-      intros.
       unfold Substable.apply_subst.
-      simpl.
-      unfold apply_subst.
+      model_crush.
       rewrite H0.
       f_equal.
       apply app_inv_tail_iff.
-      induction H.
-      trivial.
-      repeat rewrite named_map_cons_eq.
-      apply invert_eq_cons_cons; constructor.
-      simpl in H1.
-      unfold eq_term in H1.
-      rewrite H1.
-      trivial.
-      apply IHeq_subst.
+      induction H; model_crush.
     Qed.
 
   Lemma wf_term_var : forall (c : list V) (n : V),
                   In n c -> ws_term c (inj_var n).
   Proof.
-    unfold_all.
-    constructor; intros; simpl.
+    model_crush.
+    constructor; model_crush.
     - apply H1; trivial.
-    - unfold id_substable; intros.
-      apply functional_extensionality.
-      intros.
-      induction c0.
-      trivial.
-      destruct a.
-      unfold apply_subst.
-      simpl in *.
-      case_eq (eqb n v); intros.
-      apply eqb_eq in H0.
-      rewrite H0.
-      trivial.
-      apply IHc0.
+    - unfold id_substable; model_crush.
+      induction c0; model_crush.
   Qed.
 
   Lemma wf_subst_same_name : forall c' s c, wf_subst c' s c -> map fst c = map fst s.
   Proof.
-    intros.
-    induction H; trivial.
-    simpl.
-    rewrite IHwf_subst.
-    trivial.
+    model_crush.
+    induction H; model_crush.
   Qed.
 
 
@@ -437,12 +387,8 @@ Notation Model := (@Model V term sort).
         wf_subst c'' s c ->
         wf_term c'' e[/s/] t [/s/].
   Proof.
-    constructor; intros.
-    + unfold Substable.apply_subst.
-      unfold_all.
-      unfold wf_term in H.
-      apply wf_subst_same_name in H1 as Hs.
-      repeat erewrite ws_term_append; cleanup_ws_append.
+    constructor; unfold Substable.apply_subst; model_crush.
+    + repeat erewrite ws_term_append; model_crush; model_crush.
       clear H.
       f_equal.
       induction H1.
@@ -455,16 +401,11 @@ Notation Model := (@Model V term sort).
       rewrite H10.
       trivial.
       trivial.
-      eapply wf_subst_same_name; apply H1.
+      all: erewrite <- wf_subst_same_name; eauto.
     + unfold id_substable.
-      unfold Substable.apply_subst.
-      unfold_all.
-      unfold wf_term in H.
-      intros.
+      model_crush.
       apply wf_subst_same_name in H1 as Hs.
-      apply functional_extensionality; intros.
-      unfold apply_subst.
-      repeat erewrite ws_term_append; cleanup_ws_append.
+      repeat erewrite ws_term_append; model_crush; model_crush.
       f_equal.
       clear H.
       induction H1; trivial.
@@ -479,6 +420,7 @@ Notation Model := (@Model V term sort).
       trivial.
       apply wf_subst_same_name in H1.
       trivial.
+      all: erewrite <- wf_subst_same_name; eauto.
 Qed.
 
   Instance model_ok : Model_ok model.
@@ -497,3 +439,11 @@ Qed.
     + apply wf_term_subst_monotonicity with (c := c); trivial.
 Qed.
 
+Class Model_from_exp :=
+  {
+    subst_term := substable_term;
+    subst_sort := substable_sort
+  }.
+
+
+End WithExp.
